Register.v
@@ -1,7 +1,9 @@
-Require Import 
+Require Import
   List
   Nat
-  LTS.
+  Arith
+  LTS
+  LibVar.
 From VCO Require LibEnv.
 Import ListNotations.
 
@@ -86,11 +88,13 @@ Section Register.
   Inductive register_initial_state : Register_state -> Pid -> query li_register -> Register_state -> Prop :=
   | register_initial_state_cas : forall pid old new st st' inv res v,
     pid # inv -> pid # res ->
+    ok inv -> ok res ->
     st = mkRegState inv res v ->
     st' = mkRegState ((pid, RegCAS old new)::inv) res v ->
     register_initial_state st pid (RegCAS old new) st'
   | register_initial_state_read : forall pid st st' inv res v,
     pid # inv -> pid # res ->
+    ok inv -> ok res ->
     st = mkRegState inv res v ->
     st' = mkRegState ((pid, RegRead)::inv) res v ->
     register_initial_state st pid (RegRead) st'
@@ -102,11 +106,13 @@ Section Register.
   Inductive register_final_state : Register_state -> Pid -> reply li_register -> Register_state -> Prop :=
   | register_final_state_cas : forall pid inv res res' res'' b v st st',
     res = res' ++ [(pid, RegCASOk b)] ++ res'' ->
+    ok inv -> ok res ->
     st = mkRegState inv res v ->
     st' = mkRegState inv (res' ++ res'') v ->
     register_final_state st pid (RegCASOk b) st'
   | register_final_state_read : forall pid inv res res' res'' v st st' ret,
     res = res' ++ [(pid, RegReadOk ret)] ++ res'' ->
+    ok inv -> ok res ->
     st = mkRegState inv res v ->
     st' = mkRegState inv (res' ++ res'') v ->
     register_final_state st pid (RegReadOk ret) st'
@@ -118,11 +124,15 @@ Section Register.
   Inductive register_step : Register_state -> Pid -> Internal -> Register_state -> Prop :=
   | register_step_cas : forall pid st st' inv inv' inv'' res v old new,
     inv = inv' ++ [(pid, RegCAS old new)] ++ inv'' ->
+    ok inv -> ok res ->
+    pid # res ->
     st = mkRegState inv res v ->
     st' = mkRegState (inv' ++ inv'') ((pid, RegCASOk (st.(value) =? old))::res) (if value st =? old then new else old) ->
     register_step st pid int_cas st'
   | register_step_read : forall pid st st' inv inv' inv'' res v,
     inv = inv' ++ [(pid, RegRead)] ++ inv'' ->
+    ok inv -> ok res ->
+    pid # res ->
     st = mkRegState inv res v ->
     st' = mkRegState (inv' ++ inv'') ((pid, RegReadOk v)::res) v ->
     register_step st pid int_read st' 
@@ -159,3 +169,231 @@ Section Register.
   .
   
 End Register.
+
+Section Properties.
+
+Import LibEnv.
+
+Definition RegStateWF st :=
+  ok st.(requests) /\ ok st.(responses).
+
+Lemma reg_initial_preserves_ok: forall st st' pid qb,
+  initial_state Register st pid qb st' ->
+  RegStateWF st ->
+  RegStateWF st'.
+Proof.
+  inversion 1; intros; subst;
+  unfold RegStateWF; simpl; intuition;
+  econstructor; eauto.
+Qed.
+
+Lemma reg_final_state_preserves_ok: forall st st' pid rb,
+  final_state Register st pid rb st' ->
+  RegStateWF st ->
+  RegStateWF st'.
+Proof.
+  inversion 1; intros; subst;
+  unfold RegStateWF; simpl; intuition;
+  apply ok_remove in H2; intuition.
+Qed.
+
+Lemma reg_at_external_preserves_ok: forall st st' pid qa,
+  at_external Register st pid qa st' ->
+  RegStateWF st ->
+  RegStateWF st'.
+Proof.
+  inversion 1; intros; subst;
+  unfold RegStateWF; simpl; intuition;
+  apply ok_remove in H2; intuition.
+Qed.
+
+Lemma reg_after_external_preserves_ok: forall st st' pid ra,
+  after_external Register st pid ra st' ->
+  RegStateWF st ->
+  RegStateWF st'.
+Proof.
+  inversion 1; intros; subst;
+  unfold RegStateWF; simpl; intuition;
+  apply ok_remove in H2; intuition.
+Qed.
+
+Lemma reg_step_preserves_ok: forall st st' pid int,
+  step Register st pid int st' ->
+  RegStateWF st ->
+  RegStateWF st'.
+Proof.
+  inversion 1; intros; subst; simpl;
+  unfold RegStateWF; simpl; intuition;
+  apply ok_remove in H1; intuition;
+  econstructor; eauto.
+Qed.
+
+Lemma astep_preserves_ok: forall st st',
+  automaton_step Register st st' ->
+  RegStateWF st ->
+  RegStateWF st'.
+Proof.
+  intros. unfold automaton_step in H.
+  destruct H as [pid Htmp]. intuition.
+  - destruct H as [a Ha].
+    eapply reg_initial_preserves_ok; eauto.
+  - destruct H1 as [a Ha].
+    eapply reg_final_state_preserves_ok; eauto.
+  - destruct H as [a Ha].
+    eapply reg_at_external_preserves_ok; eauto.
+  - destruct H1 as [a Ha].
+    eapply reg_after_external_preserves_ok; eauto.
+  - destruct H1 as [a Ha].
+    eapply reg_step_preserves_ok; eauto.
+Qed.
+
+Lemma valid_execution_preserves_ok: forall st st' acts,
+  valid_execution_fragment Register st st' acts ->
+  RegStateWF st ->
+  RegStateWF st'.
+Proof.
+  induction 1; simpl; intros.
+  - subst; auto.
+  - eapply reg_step_preserves_ok in H; eauto.
+  - eapply reg_at_external_preserves_ok in H; eauto.
+  - eapply reg_after_external_preserves_ok in H; eauto.
+  - eapply reg_initial_preserves_ok in H; eauto.
+  - eapply reg_final_state_preserves_ok in H; eauto.
+Qed.
+  
+Lemma reachable_inv: forall st,
+  reachable Register st ->
+  RegStateWF st.
+Proof.
+  intros. unfold reachable in H.
+  destruct H as [init [acts [Hnew Hexe]]].
+  eapply valid_execution_preserves_ok; eauto.
+  inversion Hnew; subst.
+  unfold new_register.
+  unfold RegStateWF. simpl. intuition; econstructor.
+Qed.
+
+Lemma binds_same: forall (req: env Register_query) pid qb qb',
+  ok req ->
+  binds pid qb req ->
+  binds pid qb' req ->
+  qb = qb'.
+Proof.
+  induction 1; simpl; intros.
+  - inversion H.
+  - unfold binds in H1, H2. simpl in H1, H2.
+    destruct (pid =? x)eqn:Heq.
+    -- inversion H1; inversion H2; subst; auto.
+    -- apply IHok; eauto.
+Qed.
+
+Lemma internal_preserves_notin: forall acts pid st st',
+  gather_pid_external_events acts pid = [] ->
+  pid # st.(requests) ->
+  valid_execution_fragment Register st st' acts ->
+  pid # st'.(requests).
+Proof.
+  intros.
+  induction H1.
+  - subst. assumption.
+  - apply IHvalid_execution_fragment; auto.
+    eapply notin_dom_subset; eauto.
+    simpl in H1. inversion H1; subst.
+    -- simpl requests.
+      eapply subset_concat.
+      apply ok_concat_inv in H4.
+      destruct H4.
+      econstructor; eauto.
+      econstructor; eauto.
+      apply ok_concat_inv in H3. intuition.
+      intuition.
+    -- simpl requests.
+      eapply subset_concat.
+      apply ok_concat_inv in H4.
+      destruct H4.
+      econstructor; eauto.
+      econstructor; eauto.
+      apply ok_concat_inv in H3. intuition.
+      intuition.
+  - inversion H1.
+  - inversion H1.
+  - simpl in H.
+    destruct (pid =? pid0)eqn:Heq.
+    -- inversion H.
+    -- apply IHvalid_execution_fragment; auto.
+      simpl in H1.
+      inversion H1; subst.
+      + simpl requests.
+        simpl.
+        apply notin_union. intuition.
+        apply notin_neq; auto.
+        apply Nat.eqb_neq. assumption.
+      + simpl requests.
+        simpl.
+        apply notin_union. intuition.
+        apply notin_neq; auto.
+        apply Nat.eqb_neq. assumption.
+  - simpl in H.
+    destruct (pid =? pid0)eqn:Heq.
+    -- inversion H.
+    -- apply IHvalid_execution_fragment; auto.
+      simpl in H1.
+      inversion H1; subst; simpl; assumption.
+Qed.
+
+Lemma initial_preserves_binds: forall st st',.
+Proof.
+  
+Qed.
+
+
+Lemma internal_preserves_request: forall acts pid st st' qb qb',
+  gather_pid_external_events acts pid = [] ->
+  binds pid qb st.(requests) ->
+  RegStateWF st ->
+  binds pid qb' st'.(requests) ->
+  valid_execution_fragment Register st st' acts ->
+  qb = qb'.
+Proof.
+  intros. induction H3.
+  - subst. eapply binds_same; eauto.
+    unfold RegStateWF in H1; intuition.
+  - eapply IHvalid_execution_fragment; eauto.
+    destruct (pid =? pid0)eqn:Heq.
+    -- assert (pid # st'.(requests)).
+      eapply internal_preserves_notin; eauto.
+      simpl in H3.
+      apply Nat.eqb_eq in Heq. subst.
+      inversion H3; subst.
+      + simpl requests.
+        apply ok_middle_inv in H6.
+        apply notin_concat; eauto.
+      + simpl requests.
+        apply ok_middle_inv in H6.
+        apply notin_concat; eauto.
+      + apply binds_fresh_inv in H2; intuition.
+    -- simpl in H3. inversion H3; subst; simpl.
+      + simpl in H0.
+        eapply binds_remove with (E2:=[(pid0, RegCAS old new)]); simpl; eauto.
+        apply notin_neq. apply Nat.eqb_neq. assumption.
+      + simpl in H0.
+        eapply binds_remove with (E2:=[(pid0, RegRead)]); simpl; eauto.
+        apply notin_neq. apply Nat.eqb_neq. assumption.
+    -- eapply reg_step_preserves_ok; eauto.
+  - inversion H3.
+  - inversion H3.
+  - simpl in H.
+    destruct (pid =? pid0)eqn:Heq.
+    -- inversion H.
+    -- apply IHvalid_execution_fragment; auto.
+
+
+        
+    --
+
+
+
+    
+Qed.
+
+End Properties.
